src/kernelbench/level1/challenge39/Kuiper.KB.L2Norm.fsti
@@ -36,12 +36,12 @@ type l2norm_fw_ty (t:Type0) {| scalar t, real_like t, floating t |} =
   (d : szp { d <= max_blocks * max_threads /\
              SZ.fits (b * d) /\
              b * d <= max_blocks * max_threads })
-  (x : array1 t (l1_forward (b *^ d)) { is_global x })
-  (#s : chest1 t (b *^ d))
+  (x : array1 t (l1_forward (b * d)) { is_global x })
+  (#s : chest1 t (b * d))
   preserves cpu
   requires on gpu_loc (x |-> s)
   ensures
-    exists* (s' : chest1 t (b *^ d)).
+    exists* (s' : chest1 t (b * d)).
       on gpu_loc (x |-> s') **
       pure (l2norm_post (SZ.v b) (SZ.v d) (chest1_to_seq s) (chest1_to_seq s'))
 
