src/lib/kernel/Kuiper.Kernel.ConvT2D.Naive.fst
@@ -392,6 +392,7 @@ fn convt2d_naive_setup
   (b cin h_in w_in cout : szp) (kh kw : szp)
   (sh sw : szp) (ph pw : sz) (dh dw : szp)
   (h_out w_out : szp)
+  (nthr : szp { SZ.v nthr == b * cout * h_out * w_out })
   (#lx : layout1 (b * cin * h_in * w_in))
   (#lw : layout1 (cin * cout * kh * kw))
   (#lbias : layout1 cout)
@@ -415,7 +416,7 @@ fn convt2d_naive_setup
     (gbias |-> Frac fb sbias) **
     (gy |-> sy0)
   ensures
-    (forall+ (tid : natlt (b *^ cout *^ h_out *^ w_out)).
+    (forall+ (tid : natlt nthr).
        kpre #et b cin h_in w_in cout kh kw h_out w_out
             #lx #lw #lbias #ly
             gx gw gbias gy sx sw_l sbias sy0 fx fw fb tid) **
@@ -452,8 +453,7 @@ fn convt2d_naive_setup
        (gw |-> Frac (fw /. (b * cout * h_out * w_out)) sw_l) **
        (gbias |-> Frac (fb /. (b * cout * h_out * w_out)) sbias) **
        (Cell gy (idx1 i) |-> acc1 sy0 i));
-  forevery_rw_size (b * cout * h_out * w_out)
-                   (SZ.v (b *^ cout *^ h_out *^ w_out));
+  forevery_rw_size (b * cout * h_out * w_out) nthr;
   ()
 }
 
@@ -465,6 +465,7 @@ fn convt2d_naive_teardown
   (b cin h_in w_in cout : szp) (kh kw : szp)
   (sh sw : szp) (ph pw : sz) (dh dw : szp)
   (h_out w_out : szp)
+  (nthr : szp { SZ.v nthr == b * cout * h_out * w_out })
   (#lx : layout1 (b * cin * h_in * w_in))
   (#lw : layout1 (cin * cout * kh * kw))
   (#lbias : layout1 cout)
@@ -482,7 +483,7 @@ fn convt2d_naive_teardown
   ()
   norewrite
   requires
-    (forall+ (tid : natlt (b *^ cout *^ h_out *^ w_out)).
+    (forall+ (tid : natlt nthr).
        kpost #et b cin h_in w_in cout kh kw sh sw ph pw dh dw
              h_out w_out
              #lx #lw #lbias #ly
@@ -500,8 +501,7 @@ fn convt2d_naive_teardown
                               sh sw ph pw dh dw
                               h_out w_out sx sw_l sbias tid))
 {
-  forevery_rw_size (SZ.v (b *^ cout *^ h_out *^ w_out))
-                   (b * cout * h_out * w_out)
+  forevery_rw_size nthr (b * cout * h_out * w_out)
     #(kpost #et b cin h_in w_in cout kh kw sh sw ph pw dh dw
             h_out w_out
             #lx #lw #lbias #ly
@@ -596,14 +596,14 @@ let kdesc
                  convT2d_out_at b cin h_in w_in cout kh kw
                                 sh sw ph pw dh dw
                                 h_out w_out sx sw_l sbias tid)))
-=
-{
-  nthr = b *^ cout *^ h_out *^ w_out;
+  = [@@inline_let] let nthr : (x : szp { SZ.v x == b * cout * h_out * w_out }) =
+      b *^ cout *^ h_out *^ w_out in {
+  nthr = nthr;
   frame = pure (SZ.fits (tlayout_ulen ly));
   setup    = convt2d_naive_setup b cin h_in w_in cout kh kw sh sw ph pw dh dw
-                                 h_out w_out gx gw gbias gy;
+                                 h_out w_out nthr gx gw gbias gy;
   teardown = convt2d_naive_teardown b cin h_in w_in cout kh kw sh sw ph pw dh dw
-                                    h_out w_out gx gw gbias gy;
+                                    h_out w_out nthr gx gw gbias gy;
   kpre  = kpre #et b cin h_in w_in cout kh kw h_out w_out
                #lx #lw #lbias #ly gx gw gbias gy sx sw_l sbias sy0 fx fw fb;
   kpost = kpost #et b cin h_in w_in cout kh kw sh sw ph pw dh dw
